---
layout: page
title: Problem 2
mathjax: true
tags: [euler]
---

<h3 style="color: #8f5536; text-align: center">Even Fibonacci numbers</h3>

> <small><span style="font-size: 1rem; color: #90a959">Each new term in the Fibonacci sequence is generated by adding the previous two terms. By starting with 1 and 2, the first 10 terms will be: <br>
> 1, 2, 3, 5, 8, 13, 21, 34, 55, 89, ... <br>
> By considering the terms in the Fibonacci sequence whose values do not exceed four million, find the sum of the even-valued terms.</span><br><br>
> <cite>[http://projecteuler.net/problem=2](http://projecteuler.net/problem=2)</cite></small>
{: style="background-color: #2d2d2d"}

#### Brute Force

{% highlight Javascript %}
function euler2() {
  var sum = 0,
      fn = 1,
      fm = 1; // f n-1
  while (fn < 4000000) {
    if (fn % 2 === 0) {
      sum += fn;
    }
    fn = fn + fm;
    fm = fn - fm;
  }
  return sum;
}
timer(euler2, 100000);
// euler2 x 100000: 16.298ms
// 4613732

# Time O(n)
{% endhighlight %}


#### Patterns

Let's take a look at the values of the sequence.

{% highlight Javascript %}
var n = 1,
    fn = 1,
    fm = 0; // f n-1
while (n < 25) {
  console.log('n', n, 'fib', fn, fn%2 === 0 ? 'even' : '');
  fn = fn + fm;
  fm = fn - fm;
  n++;
}

n 1 fib 1
n 2 fib 1
n 3 fib 2 even
n 4 fib 3
n 5 fib 5
n 6 fib 8 even
n 7 fib 13
n 8 fib 21
n 9 fib 34 even
n 10 fib 55
n 11 fib 89
n 12 fib 144 even
n 13 fib 233
n 14 fib 377
n 15 fib 610 even
n 16 fib 987
n 17 fib 1597
n 18 fib 2584 even
n 19 fib 4181
n 20 fib 6765
n 21 fib 10946 even
n 22 fib 17711
n 23 fib 28657
n 24 fib 46368 even
{% endhighlight %}

What we can see is that $F_3$, $F_6$, $F_9$, ... $F_{(n\,multiple\,of\,3)}$ are the even fibonacci numbers.

Using this is a bit of information is going to take some manipulation. A fibonacci number can be generalized as:

$$F_n = F_{n-1} + F_{n-2}$$

----

Using $$F_{n-1} = F_{n-2} + F_{n-3}$$ to replace $$F_{n-1}$$ we get:

$$F_n = (F_{n-2} + F_{n-3}) + F_{n-2} = 2F_{n-2} + F_{n-3}$$

----

Using $$F_{n-2} = F_{n-3} + F_{n-4}$$ to replace $$F_{n-2}$$ we get:

$$F_n = 2F_{n-3} + 2F_{n-4} + F_{n-3} = 3F_{n-3} + 2F_{n-4}$$

----

Using $$F_{n-4} = F_{n-5} + F_{n-6}$$ to replace a single $$F_{n-4}$$ we get:

$$F_n = 3F_{n-3} + F_{n-4} + F_{n-5} + F_{n-6}$$

----

Going the other way, replacing $$F_{n-4} + F_{n-5}$$ with $$F_{n-3}$$ we get:

$$F_n = 3F_{n-3} + F_{n-3} + F_{n-6} = 4F_{n-3} + F_{n-6}$$

----

For example:

$$F_6 = 4F_3 + F_0 = 4\times2 + 0 = 8$$

We can use this to solve our problem!

#### Better Brute Force

{% highlight Javascript %}
function euler2() {
  var sum = 0,
      fa = 2, // f n-3
      fb = 0; // f n-6
  while (fa < 4000000) {
    sum += fa;
    fa = 4*fa + fb;
    fb = (fa - fb) / 4;
  }
  return sum;
}
timer(euler2, 100000);
// euler2 x 100000: 8.252ms
// 4613732

# Time O(n)
{% endhighlight %}

We are using a trick to set the new value of the $$F_{n-6}$$ variable, `fb`. We want to set `fb` to $$F_{n-3}$$, but the variable we were using for $$F_{n-3}$$, `fa` has been set to $$F_{n}$$. We can use our knowledge that $$F_{n-3} = \frac{F_{n} - F_{n-6}}4$$ and set `fb` to `(fa - fb) / 4`.
